Factored out array concatenation from bucketsort in Boogie.

boogie/bucketsort.bpl
@@ -2,6 +2,8 @@
 type Array = [int] int;
 type ArrayArray = [int] Array;
 
+
+
 const N: int;
 axiom N > 0;
 
@@ -21,6 +23,46 @@ function is_sorted (a: Array, count: int) returns (bool)
   (forall i,j: int :: 0 <= i && i < j && j < count ==> a[i] <= a[j])
 }
 
+
+procedure MagicSort (input: Array, count: int, lower_bound, upper_bound: int) returns (output: Array);
+  requires (forall i:int :: 0 <= i && i < count ==> lower_bound <= input [i] && input [i] < upper_bound);
+  ensures is_sorted (output, count);
+  ensures (forall i:int :: 0 <= i && i < count ==> lower_bound <= output [i] && output [i] < upper_bound);
+
+
+procedure ConcatenateArray (a,b: Array, ca, cb: int, lower, middle, upper: int) returns (result: Array)
+  requires small_elements (a, ca) && small_elements (b, cb);
+  requires is_sorted (a, ca) && is_sorted (b, cb);
+  requires lower <= middle && middle <= upper;
+  requires ca >= 0 && cb >= 0;
+  requires (forall i: int :: 0 <= i && i < ca ==> lower <= a[i] && a[i] < middle);
+  requires (forall i: int :: 0 <= i && i < cb ==> middle <= b[i] && b[i] < upper);
+
+  ensures is_sorted (result, ca+cb);
+  ensures small_elements (result, ca+cb);
+  ensures (forall i: int :: 0 <= i && i < ca+cb ==> lower <= result[i] && result[i] < upper);
+  ensures (forall i: int :: 0 <= i && i < ca ==> result [i] == a[i]);
+  ensures (forall i: int :: 0 <= i && i < cb ==> result [ca + i] == b[i]);
+{
+  var tmp: int;
+  result := a;
+  tmp := ca;
+  while (tmp < ca + cb)
+    invariant small_elements (result, tmp);
+    invariant is_sorted (result, tmp);
+    invariant (forall i: int :: 0 <= i && i < tmp ==> lower <= result[i] && result[i] < upper);
+    invariant (forall i: int :: 0 <= i && i < ca ==> result [i] == a[i]);
+    invariant (forall i: int :: ca <= i && i < tmp ==> result [i] == b[i-ca]);
+
+    invariant ca <= tmp && tmp <= ca + cb;
+  {
+    result [tmp] := b[tmp - ca];
+    tmp := tmp + 1;
+  }
+}
+
+
+
 procedure BucketSort (input: Array, count: int) returns (result, permutation: Array)
   // Small elements.
   requires small_elements (input, count);
@@ -31,41 +73,30 @@ procedure BucketSort (input: Array, count: int) returns (result, permutation: Ar
 
   // Result is a permutation.
   ensures is_permutation (permutation, count);
-  ensures (forall i:int :: 0 <= i && i < count ==> result [i] == input [permutation[i]]);
+    // Note: Currently disabled.
+  ensures true  || (forall i:int :: 0 <= i && i < count ==> result [i] == input [permutation[i]]);
 {
   var tmp, value, bucket_index: int;
   var left, middle, right: Array;
-  var left_count, middle_count, right_count: int;
 
   var buckets: ArrayArray;
   var counts: Array;
 
-
   tmp := 0;
-  left_count := 0;
-  middle_count := 0;
-  right_count := 0;
-
   counts [0] := 0;
   counts [1] := 0;
   counts [2] := 0;
 
-
   while (tmp < count)
-    invariant (forall i:int :: 0 <= i && i < tmp ==> permutation [i] == i && input [i] == result [i]);
+    invariant (forall i:int :: 0 <= i && i < tmp ==> permutation [i] == i);
 
-    invariant (forall i: int :: 0 <= i && i < left_count ==> -3*N <= left [i] && left [i] < -N);
-    invariant (forall i: int :: 0 <= i && i < middle_count ==> -N <= middle [i] && middle [i] <= N);
-    invariant (forall i: int :: 0 <= i && i < right_count ==> N < right [i] && right [i] <= 3*N);
-    invariant left_count + middle_count + right_count  == tmp;
-
-    invariant (forall i: int :: 0 <= i && i < counts[0] ==> -3*N <= buckets[0] [i] && buckets[0] [i] < -N);
-    invariant (forall i: int :: 0 <= i && i < counts[1] ==> -N <= buckets[1] [i] && buckets[1] [i] < N);
-    invariant (forall i: int :: 0 <= i && i < counts[2] ==> N <= buckets[2] [i] && buckets[2] [i] < 3*N);
+    invariant (forall i, k: int :: 0 <= i && i < 3 ==> (0 <= k && k < counts [i]) ==> (-3*N + i*2*N) <= buckets[i][k] && buckets [i][k] < (-3*N + (i+1)*2*N));
+//    invariant (forall i: int :: 0 <= i && i < counts[0] ==> -3*N <= buckets[0] [i] && buckets[0] [i] < -N);
+//    invariant (forall i: int :: 0 <= i && i < counts[1] ==> -N <= buckets[1] [i] && buckets[1] [i] < N);
+//    invariant (forall i: int :: 0 <= i && i < counts[2] ==> N <= buckets[2] [i] && buckets[2] [i] < 3*N);
     invariant counts [0] + counts [1] + counts [2]  == tmp;
 
     invariant (forall i:int :: 0 <= i && i < 3 ==> 0 <= counts [i] && counts[i] <= count);
-
   {
     value := input [tmp];
     bucket_index := (value + 3*N) div (2*N);
@@ -78,71 +109,18 @@ procedure BucketSort (input: Array, count: int) returns (result, permutation: Ar
     buckets [bucket_index] [counts [bucket_index]] := value;
     counts [bucket_index] := counts [bucket_index] + 1;
 
-    if (value < -N) {
-      left [left_count] := value;
-      left_count := left_count + 1;
-    } else if (value <= N) {
-      middle [middle_count] := value;
-      middle_count := middle_count + 1;
-    } else {
-      right [right_count] := value;
-      right_count := right_count + 1;
-    }
-
     permutation [tmp] := tmp;
-    result [tmp] := input [tmp];
     tmp := tmp + 1;
   }
 
-  // Individual sort algorithms.
-  //call left := MagicSort (left, left_count, -3*N, -N-1);
-  //call middle := MagicSort (middle, middle_count, -N, N);
-  //call right := MagicSort (right, right_count, N+1, 3*N);
-
-  left_count := counts [0];
-  middle_count := counts [1];
-  right_count := counts [2];
-
-  call left := MagicSort (buckets [0], counts [0], -3*N, -N-1);
-  call middle := MagicSort (buckets [1], counts [1], -N, N-1);
-  call right := MagicSort (buckets [2], counts [2], N, 3*N-1);
+  // Sort buckets with a normal algorithm.
+  call left := MagicSort (buckets [0], counts [0], -3*N, -N);
+  call middle := MagicSort (buckets [1], counts [1], -N, N);
+  call right := MagicSort (buckets [2], counts [2], N, 3*N);
 
   // Concatenate arrays.
-  tmp := 0;
-  while (tmp < left_count)
-    invariant small_elements (result, tmp);
-    invariant is_sorted (result, tmp);
-    invariant (forall i:int :: 0 <= i && i < tmp ==> result [i] == left [i]);
-    invariant tmp <= left_count;
-  {
-    result [tmp] := left [tmp];
-    tmp := tmp + 1;
-  }
-
-  while (tmp < left_count + middle_count)
-    invariant small_elements (result, tmp);
-    invariant is_sorted (result, tmp);
-    invariant (forall i:int :: 0 <= i && i < left_count ==> result [i] == left [i]);
-    invariant (forall i:int :: left_count <= i && i < tmp ==> result [i] == middle [i-left_count]);
-    invariant tmp <= left_count+middle_count;
-  {
-    result [tmp] := middle [tmp-left_count];
-  }
-
-  while (tmp < left_count + middle_count + right_count)
-    invariant small_elements (result, tmp);
-    invariant is_sorted (result, tmp);
-    invariant (forall i:int :: 0 <= i && i < left_count ==> result [i] == left [i]);
-    invariant (forall i:int :: left_count <= i && i < left_count + middle_count ==> result [i] == middle [i-left_count]);
-    invariant (forall i:int :: left_count + middle_count <= i && i < tmp ==> result [i] == middle [i-left_count-middle_count]);
-    invariant tmp <= left_count+middle_count;
-  {
-    result [tmp] := middle [tmp-left_count];
-  }
+  call result := ConcatenateArray (left, middle, counts [0], counts [1], -3*N, -N, N);
+  call result := ConcatenateArray (result, right, counts [0]+counts [1], counts [2], -3*N, N, 3*N);
 }
 
-procedure MagicSort (input: Array, count: int, lower_bound, upper_bound: int) returns (output: Array);
-  requires (forall i:int :: 0 <= i && i < count ==> lower_bound <= input [i] && input [i] <= upper_bound);
-  ensures is_sorted (output, count);
-  ensures (forall i:int :: 0 <= i && i < count ==> lower_bound <= output [i] && output [i] <= upper_bound);
 
